\documentclass[a4paper, 11pt]{article}
\input{../preamble.tex}
\title{Math 20250: Abstract Linear Algebra \\ \large Problem Set 2}
\date{09 Apr 2023}
\author{Hung Le Tran}
\begin{document}
\maketitle
\newpage
\setcounter{section}{2}
\textbf{Textbook: Linear Algebra by Hoffman and Kunze (2nd Edition)}
\begin{problem} [Sec 2.2. Problem 3]
Is the vector \((3, -1, 0, -1)\) in the subspace of \(\bbr^5\) spanned by the vectors \((2, -1, 3, 2), (-1, 1, 1, -3)\) and \((1, 1, 9, -5)\)?
\end{problem}
\begin{solution}
    For \((3, -1, 0, -1)\) to be in the abovementioned subspace, it must be a linear combination of the vectors \((2, -1, 3, 2), (-1, 1, 1, -3) \:\text{and}\: (1, 1, 9, -5)\) in \(\bbr^5\), i.e. \[
        \exists c_1, c_2, c_3 \in \bbr \st (3, -1, 0, -1) = c_1(2, -1, 3, 2) + c_2(-1, 1, 1, -3) + c_3(1, 1, 9, -5)
    \]

    It follows that
    \begin{align*}
        2c_1 -c_2 + c_3   & =3   \\
        -c_1 + c_2 + c_3  & = -1 \\
        3c_1 + c_2 + 9c_3 & = 0  \\
        2c_1 -3c_2 -5c_3  & = -1
    \end{align*}
    which is equivalent to:
    \[
        \left[\begin{array}{ccc}
                2  & -1 & 1  \\
                -1 & 1  & 1  \\
                3  & 1  & 9  \\
                2  & -3 & -5
            \end{array}\right]\left[\begin{array}{c}
                c_1 \\
                c_2 \\
                c_3
            \end{array}\right] = \left[\begin{array}{c}
                3  \\
                -1 \\
                0  \\
                -1
            \end{array}\right]
    \]
    which is then equivalent to the following augmented matrix:
    \[
        \left[\begin{array}{cccc}
                2  & -1 & 1  & 3  \\
                -1 & 1  & 1  & -1 \\
                3  & 1  & 9  & 0  \\
                2  & -3 & -5 & -1
            \end{array}\right]
    \]

    on which we can carry out simplifying row operations to reach the row-reduced echelon form:
    \[
        \left[\begin{array}{cccc}
                1 & 0 & 2 & 0 \\
                0 & 1 & 3 & 0 \\
                0 & 0 & 0 & 1 \\
                0 & 0 & 0 & 0
            \end{array}\right]
    \]

    The system therefore has no solution, as the third row of the augmented matrix fails (\(0c_1 + 0c_2 + 0c_3 \neq 1\))

    Therefore \((3, -1, 0, 1)\) is not in the subspace.
\end{solution}

\begin{problem} [Sec 2.2. Problem 5]
Let \(\bbf\) be a field and let \(n \geq 2\) be a positive integer. Let \(V\) be the vector space of all \(n \times n\) matrices over \(\bbf\). Which of the following sets of matrices \(A \in V\) are subspaces of \(V\)?
\begin{enumerate}
    \item all invertible \(A\)
    \item all non-invertible \(A\)
    \item all \(A \st AB = BA\), where \(B\) is some fixed matrix in \(V\)
    \item all \(A \st A^2 = A\)
\end{enumerate}
\end{problem}
\begin{solution}
    \begin{enumerate}
        \item All invertible \(A\)

              No. It is not true that \(\forall \:\text{invertible}\: A_1, A_2 \in V, (A_1 + A_2)\) is also invertible.

              Counter example: \[
                  A_1 = \left[\begin{array}{cc}
                          1 & 0 \\
                          0 & 1
                      \end{array}\right], A_2 = \left[\begin{array}{cc}
                          0 & 1 \\
                          1 & 0
                      \end{array}\right] \implies A_3 = A_1 + A_2 = \left[\begin{array}{cc}
                          1 & 1 \\
                          1 & 1 \\
                      \end{array}\right]
              \]

              which is not invertible, since it admits \(X = \left[\begin{array}{c}
                      a \\ -a
                  \end{array}\right]\) for arbitrary \(a \in \bbf\) as a solution to \(A_3X = 0\)

        \item All non-invertible \(A\)

              No. It is not true that \(\forall \:\text{non-invertible}\: A_1, A_2 \in V, (A_1 + A_2)\) is also non-invertible.

              Counter example: \[
                  A_1 = \left[\begin{array}{cc}
                          1 & 0 \\
                          0 & 0
                      \end{array}\right], A_2 = \left[\begin{array}{cc}
                          0 & 0 \\
                          0 & 1
                      \end{array}\right] \implies A_3 = A_1 + A_2 = \left[\begin{array}{cc}
                          1 & 0 \\
                          0 & 1 \\
                      \end{array}\right]
              \]

              \(A_1\) is non-invertible since it admits \(X = \left[\begin{array}{c}
                      0 \\ a
                  \end{array}\right]\) for arbitrary \(a \in \bbf\) as a solution to \(A_1X = 0\)

              \(A_2\) is non-invertible since it admits \(X = \left[\begin{array}{c}
                      a \\ 0
                  \end{array}\right]\) for arbitrary \(a \in \bbf\) as a solution to \(A_2X = 0\)

              Meanwhile, \(A_3 = I\) is trivially invertible.

        \item All \(A \st AB = BA\), \(B\) is fixed in \(V\)

              Yes. We want to show that given \(A_1, A_2 \st A_1B = BA_1, A_2B = BA_2\) then
              \begin{align*}
                  (A_1 + A_2)B & = B(A_1 + A_2)                 \\
                  (c A_1) B    & = B (c A_1) \forall c \in \bbk
              \end{align*}

              First, we have:
              \begin{align*}
                  [(A_1 + A_2)B]_{ij} & = \sum_{k=1}^{n}(A_1 + A_2)_{ik}B_{kj}                              \\
                                      & = \sum_{k=1}^{n}(A_{1, ik}B_{kj} + A_{2, ik}B_{kj})                 \\
                                      & = \sum_{k=1}^{n}(A_{1, ik}B_{kj}) + \sum_{k=1}^{n}(A_{2, ik}B_{kj}) \\
              \end{align*}

              However, \[
                  A_1B = BA_1 \implies \sum_{k=1}^{n}(A_{1, ik}B_{kj}) = [A_1B]_{ij} = [BA_1]_{ij} = \sum_{k=1}^{n}(B_{ik}A_{1, kj})
              \]
              and similarly for \(A_2\).

              It follows that:
              \begin{align*}
                  [(A_1 + A_2)B]_{ij} & =\sum_{k=1}^{n}(A_{1, ik}B_{kj}) + \sum_{k=1}^{n}(A_{2, ik}B_{kj})  \\
                                      & = \sum_{k=1}^{n}(B_{ik}A_{1, kj}) + \sum_{k=1}^{n}(B_{ik}A_{2, kj}) \\
                                      & = \sum_{k=1}^{n}B_{ik}(A_{1, kj} + A_{2, kj})                       \\
                                      & = \sum_{k=1}^{n}B_{ik}(A_1 + A_2)_{kj}                              \\
                                      & = [B(A_1 + A_2)]_{ij}
              \end{align*}

              It follows that indeed \((A_1 + A_2) B = B(A_1 + A_2)\).

              The other equality is trivially observed \((c A_1) B = B (c A_1) \forall c \in \bbk\), making this set a subspace of \(V\)


        \item All \(A \st A^2 = A\)

              No. It is not true that \(\forall A_1, A_2 \st A_1^2 = A_1, A_2^2 = A_2 \implies (A_1 + A_2)^2 = A_1 + A_2\)

              Counterexample: \(A_1 = \left[\begin{array}{cc}
                      1 & 1 \\
                      0 & 0
                  \end{array}\right], A_2 = \left[\begin{array}{cc}
                      0 & 0 \\
                      0 & 1
                  \end{array}\right]\)

              It is trivially true that \(A_1^2 = A^1, A_2^2 = A_2\), however \[
                  (A_1 + A_2)^2 = \left[\begin{array}{cc}
                          1 & 1 \\
                          0 & 1
                      \end{array}\right]\left[\begin{array}{cc}
                          1 & 1 \\
                          0 & 1
                      \end{array}\right] = \left[\begin{array}{cc}
                          1 & 2 \\
                          0 & 1
                      \end{array}\right] \neq (A_1 + A_2)
              \]

              Therefore this set is not a subspace of \(V\).
    \end{enumerate}

\end{solution}

\begin{problem} [Sec 2.3. Problem 1]
Prove that if two vectors are linearly dependent, one of them is a scalar multiple of the other.
\end{problem}
\begin{solution}
    Let \(v_1, v_2\) be two vectors that are linearly dependent in field \(\bbk\). Then there exists \(a_1, a_2 \in \bbk\) not all 0 s.t.
    \begin{equation*}
        a_1v_1 + a_2v_2 = 0
    \end{equation*}

    WLOG, assume \(a_1 \neq 0 \implies \exists a_1^{-1}: a_1^{-1}a_1 = 1\). It follows that \[
        v_1 = a_1^{-1}(-a_2v_2) = (-a_1^{-1}a_2)v_2
    \]
    is a scalar multiple of \(v_2\).
\end{solution}

\begin{problem} [Sec 2.3. Problem 2]
Are the vectors
\begin{align*}
    \alpha_1 & = (1, 1, 2, 4)   \\
    \alpha_2 & = (2, -1, -5, 2) \\
    \alpha_3 & = (1, -1, 4, 0)  \\
    \alpha_4 & = (2, 1, 1, 6)
\end{align*}
linearly independent in \(\bbr^4\)?
\end{problem}
\begin{solution}
    No, because \[
        \alpha_4 = (2, 1, 1, 6) = \frac{4}{3} (1, 1, 2, 4) + \frac{1}{3} (2, -1, -5, 2) = \frac{4}{3} \alpha_1 + \frac{1}{3} \alpha_2 + 0\alpha_3
    \]
\end{solution}

\begin{problem} [Sec 2.3. Problem 4]
Show that the vectors \[
    \alpha_1 = (1, 0, -1), \alpha_2 = (1, 2, 1), \alpha_3 = (0, -3, 2)
\]
form a basis for \(\bbr^3\). Express each of the standard basis vectors as linear combinations of \(\alpha_1, \alpha_2, \alpha_3\)
\end{problem}
\begin{solution}
    We first express each of the standard basis vectors as linear combinations of \(\alpha_1, \alpha_2, \alpha_3\):
    \begin{align*}
        (1, 0, 0) & = \frac{7}{10} (1, 0, -1) + \frac{3}{10} (1, 2, 1) + \frac{1}{5} (0, -3, 2)  \\
        (0, 1, 0) & = \frac{-1}{5} (1, 0, -1) + \frac{1}{5} (1, 2, 1) + \frac{-1}{5} (0, -3, 2)  \\
        (0, 0, 1) & = \frac{-3}{10} (1, 0, -1) + \frac{3}{10} (1, 2, 1) + \frac{1}{5} (0, -3, 2) \\
    \end{align*}

    The standard basis vectors span \(V\), therefore each vector in \(V\) can be expressed as linear combinations of the standard basis vectors, which can then be expressed as linear combinations of \(\alpha_1, \alpha_2, \alpha_3\) per the equalities above. Therefore \(\alpha_1, \alpha_2, \alpha_3\) span \(V\).

    It must now be proven that they are linearly independent, which is equivalent to showing that the system of linear equations represented by the following augmented matrix has no non-trivial solutions:
    \[
        \left[\begin{array}{cccc}
                1  & 1 & 0  & 0 \\
                0  & 2 & -3 & 0 \\
                -1 & 1 & 2  & 0 \\
            \end{array}\right]
    \]

    Indeed, its row-reduced echelon form is \(\left[\begin{array}{cccc}
            1 & 0 & 0 & 0 \\
            0 & 1 & 0 & 0 \\
            0 & 0 & 1 & 0
        \end{array}\right]\), only allowing for a trivial solution of \((0, 0, 0)\). Thus, \(\alpha_1, \alpha_2, \alpha_3\) are linearly independent.

    Therefore they form a basis for \(V\).
\end{solution}

\begin{problem} [(Bonus) Sec 2.3. Problem 14]
Let \(V\) be the set of real numbers. Regard \(V\) as a vector space over the field of \textit{rational} numbers, with the usual operations. Prove that this vector space is \textit{not} finite-dimensional.
\end{problem}
\begin{solution}
    Suppose not; that \(\dim_\bbq \bbr = d \in \bbn\), meaning that there exists a basis \(v_1, v_2, \dots, v_d \in \bbr\) such that \[
        \forall v \in \bbr \exists \alpha_1, \alpha_2, \dots, \alpha_d \in \bbq: v = \alpha_1v_1 + \dots + \alpha_dv_d
    \]
    We first observe that for \(v_1 \neq v_2 \in \bbr\), their corresponding \(d-\)tuple must be different,

    i.e. \((\alpha_{v_1, 1}, \alpha_{v_2, 1}, \dots, \alpha_{v_1, d}) \neq (\alpha_{v_2, 1}, \alpha_{v_2, 2}, \dots, \alpha_{v_2, d})\). This is trivial.

    Therefore if we consider \(\phi: \bbr \to \bbq^d, \phi(v) = (\alpha_{v, 1}, \alpha_{v_2}, \dots, \alpha_{v, d})\) then \(\phi\) is injective. 

    It follows that \(\abs{\bbr} \leq \abs{\bbq^d}\). However, \(\bbr\) is uncountable and \(\bbq^d\) is countable. \contra
\end{solution}
\end{document}